montgomery arithmetic started

examples/ecAdd/proofs/AlmostYUL.ec
@@ -1,13 +1,18 @@
 require import AllCore Int IntDiv.
 
+op R2_MOD_P : int.
+op R, N, N' : int.
+
+op getHighestHalfOfMultiplication (a b : int) : int = (a * b) %/ R.
+
 
 module AlmostYul = {
 
 
-   proc overflowingAdd(augend : int, addend : int, R : int) : int * bool = {
-     var sum <- (augend + addend) %% R;
-     return (sum, sum < augend);
-   }
+  proc overflowingAdd(augend : int, addend : int, R : int) : int * bool = {
+    var sum <- (augend + addend) %% R;
+    return (sum, sum < augend);
+  }
 
   proc _REDC(Tlo : int, Thi : int, R : int, N : int, N' : int) = {
     var m, hi, lo, s, tmp, overflowed;
@@ -31,5 +36,44 @@ module AlmostYul = {
   } 
 
 
+
+  proc outOfMontgomeryForm(m : int) : int = {
+      var ret;
+      ret <@ _REDC(m, 0, R, N, N');
+      return ret;
+  } 
+
+  proc intoMontgomeryForm(a : int) : int = {
+      var ret, hi, lo;
+
+      hi <- getHighestHalfOfMultiplication a R2_MOD_P;
+      lo <- (a * R2_MOD_P) %% R;
+      ret <@ _REDC(lo, hi, R, N, N');
+    
+      return ret;
+  }
+
+  proc montgomeryAdd(augend : int, addend : int) : int = {
+    var ret;
+    ret <- (augend + addend) %% R;
+    ret <- if N <= ret then (ret - N) %% R else ret;
+    return ret;
+  }
+
+
+  proc montgomerySub(minuend : int, subtrahend : int) : int = {
+      var ret;
+      ret <@ montgomeryAdd(minuend, (N - subtrahend) %% R);
+      return ret;
+  }
+
+  proc montgomeryMul(multiplicand : int, multiplier : int) : int = {
+    var higherHalfOfProduct, lowestHalfOfProduct, ret;
+    
+    higherHalfOfProduct <- getHighestHalfOfMultiplication multiplicand multiplier;
+    lowestHalfOfProduct <- (multiplicand * multiplier) %% R;
+    ret <@ _REDC(lowestHalfOfProduct, higherHalfOfProduct, R, N, N');
+    return ret;
+  }
 
 }.
