examples/ecAdd/proofs/montgomery_arith.ec
@@ -1,0 +1,168 @@
+pragma Goals:printall.
+require import AllCore Int IntDiv.
+require import Gcd Gcd_props Opt_redc.
+
+require import AlmostYUL.
+
+
+op P = AlmostYUL.N.
+axiom ax1 : 2 * P < R.
+axiom ax2 : 0 < P.
+axiom ax3 :  N' * P %% R = (-1) %% R.
+axiom ax4 :  coprime P R.
+axiom R_pos : 0 < R. 
+axiom ax5 : 0 <= R2_MOD_P < P.
+axiom ax6 : R2_MOD_P = (R * R) %% P.
+
+op comb (l h : int) = h * R + l.
+
+lemma comb_lemma l h : 0 <= l < R => 0 <= h <= P - 1 => comb l h < R * P.
+progress.   
+rewrite /comb. 
+have f : h * R <= (P * R - R). smt.
+have q : l < R. smt.
+smt.
+qed.
+    
+
+lemma almost_yul_redc_full_correctness':
+  forall (Tlo Thi R_in N' N : int),
+    2 * N < R_in =>
+    0 < N =>
+    N' * N %% R_in = (-1) %% R_in =>
+    coprime N R_in =>
+    phoare[ AlmostYul._REDC :
+                 0 <=(comb Tlo Thi) < R_in * N /\ arg = (Tlo, Thi, R_in, N, N') ==> res = (comb Tlo Thi) * inv N R_in %% N] = 1%r.
+admitted.
+
+
+lemma qq (x a b : int) : 0 < b < a => 0  <= x =>
+     x %/ a <= x %/b. smt.
+qed.
+
+
+
+
+lemma into_m m_in :
+    phoare [ AlmostYul.intoMontgomeryForm : arg = m_in  /\ 0 <= a < P ==> res = (m_in * R) %% P ] = 1%r.
+proof. proc.
+progress.
+seq 1 : (#pre /\ hi = a * R2_MOD_P %/ R ). auto. auto.
+seq 1 : (#pre /\ lo = a * R2_MOD_P %% R). auto. auto.
+exists* lo, hi. elim*. move => loL hiL.
+simplify.
+call  (almost_yul_redc_full_correctness' loL hiL  R N' P). smt. smt. smt. smt.
+skip. progress.
+rewrite /comb. smt.
+apply comb_lemma.
+split. smt. smt.
+split. smt.
+progress.
+have q1 : a{hr} * R2_MOD_P %/ R <= a{hr} * R2_MOD_P %/ (2 * P). apply qq. smt.
+smt.
+have q2 : a{hr} * R2_MOD_P %/ (2 * P) <= a{hr}  %/ 2 . smt.
+have q3 : a{hr}  %/ 2 <= P - 1 .  smt.
+smt.
+rewrite /comb.
+have ->: (a{hr} * R2_MOD_P %/ R * R + a{hr} * R2_MOD_P %% R)
+ = (a{hr} * R2_MOD_P). smt.
+rewrite ax6.
+have ->: a{hr} * (R * R %% Top.P) * inv Top.P R
+ = a{hr} * ((R * R %% Top.P) * inv Top.P R). smt.
+
+have ->: a{hr} * (R * R %% Top.P * inv Top.P R) %% Top.P
+ = a{hr} %% Top.P * (R * R %% Top.P * inv Top.P R %% Top.P) %% Top.P. smt(@Int @IntDiv).
+admit.
+
+hoare. simplify. auto. auto.
+hoare. simplify. auto. auto.
+qed. 
+
+
+lemma outof_m m_in :
+    phoare [ AlmostYul.outOfMontgomeryForm : arg = m_in  /\ 0 <= m < P ==> res = m_in * (inv P R) %% P ] = 1%r.
+proc.
+exists* m. elim*. move => mL.
+simplify.
+call  (almost_yul_redc_full_correctness' mL 0  R N' P). smt. smt. smt. smt.
+skip. progress. smt. smt.
+qed.    
+
+
+
+lemma add_m a_in b_in :
+    phoare [ AlmostYul.montgomeryAdd : arg = (a_in,b_in)  /\ 0 <= a_in < P
+      /\  0 <= b_in <= P ==> res = (a_in + b_in) %% P ] = 1%r.
+proof. proc.
+wp. skip. progress.
+case (AlmostYUL.N <= (augend{hr} + addend{hr}) %% R).
+have f1 : (augend{hr} + addend{hr}) < 2 * P. smt.
+have f2 : (augend{hr} + addend{hr}) %% R = (augend{hr} + addend{hr}) . smt.
+rewrite f2.
+progress.
+have f3 : 0 <= (augend{hr} + addend{hr} - P) < P. split. smt.
+progress.   smt. 
+have -> : (augend{hr} + addend{hr} - AlmostYUL.N) %% R = (augend{hr} + addend{hr} - AlmostYUL.N). smt.
+progress. rewrite /P.
+smt (pmod_small @IntDiv).
+progress.
+have ->: (augend{hr} + addend{hr}) %% R = (augend{hr} + addend{hr}). smt.
+smt.
+qed.
+    
+
+
+lemma sub_m a_in b_in :
+    phoare [ AlmostYul.montgomerySub : arg = (a_in,b_in)  /\ 0 <= a_in < P
+      /\  0 <= b_in < P ==> res = (a_in - b_in) %% P ] = 1%r.
+proof. proc.
+exists* minuend, subtrahend. elim*. move => m1 m2.
+call (add_m m1 ((P - m2) %% R)). skip. progress.
+smt. smt.
+have ->: (P - subtrahend{hr}) %% R = (P - subtrahend{hr}). smt.
+smt(@Int @IntDiv).
+qed.
+
+lemma mul_m a_in b_in :
+       phoare [ AlmostYul.montgomeryMul : arg = (a_in * R %% P,b_in * R %% P)  /\ 0 <= arg.`1 < P
+         /\  0 <= arg.`2 < P ==> res = (a_in * b_in) * R %% P ] = 1%r.
+proc.
+seq 2 : (#pre /\ higherHalfOfProduct = ((a_in * R %% P) * (b_in * R %% P)) %/ R /\ lowestHalfOfProduct = ((a_in * R %% P) * (b_in * R %% P)) %% R).
+auto. wp. skip. progress.
+exists* lowestHalfOfProduct, higherHalfOfProduct. elim*.
+move => lo hi.
+call  (almost_yul_redc_full_correctness' lo hi  R N' P). smt. smt. smt. smt.
+skip. progress. 
+smt.
+have ->: comb (a_in * R %% P * (b_in * R %% P) %% R)
+  (a_in * R %% P * (b_in * R %% P) %/ R)
+   = a_in * R %% P * (b_in * R %% P). smt.
+smt.
+have ->: comb (a_in * R %% P * (b_in * R %% P) %% R)
+  (a_in * R %% P * (b_in * R %% P) %/ R)
+   = a_in * R %% P * (b_in * R %% P). smt.
+have ->:
+   a_in * R %% P * (b_in * R %% P) * inv P R %% P
+ =  a_in * R  * ((b_in * R %% P) * inv P R) %% P.
+ smt(@Int @IntDiv).
+have ->: a_in * R  * ((b_in * R %% P) * inv P R) %% P
+  = a_in * R  * ((b_in * R %% P) * inv P R %% P) %% P.
+ smt(@Int @IntDiv).  
+have ->: ((b_in * R %% P) * inv P R %% P)
+  = (b_in * R) * inv P R %% P . 
+ smt(@Int @IntDiv).  
+have ->: (b_in * R) * inv P R %% P
+ = b_in * (R * inv P R) %% P.
+smt.
+have ->: b_in * (R * inv P R) %% P 
+ = b_in * (R * inv P R %% P) %% P.
+ smt(@Int @IntDiv).
+have ->: (R * inv P R %% P) = 1.
+   smt.
+have ->: b_in * 1 = b_in. smt().
+have ->: a_in * R * (b_in %% P) %% P
+  = a_in * R * (b_in ) %% P.
+ smt(@Int @IntDiv).
+smt().
+hoare. simplify. wp. skip. progress. auto.
+qed.  
